src/Utils/Booleans.v
@@ -1,7 +1,28 @@
 Require Export Datatypes.List (forallb2).
 Require Export Datatypes.Bool.
 
-Require Import Utils.Base.
+Require Import Utils.Base Utils.Default.
+
+(*TODO: move to Booleans or a new file *)
+Definition compute_checked {b A} : (Is_true b -> A) -> option A :=
+  if b as b return (Is_true b -> _) -> _
+  then fun f => Some (f I)
+  else fun _ => None.
+
+(*TODO: move to Booleans or a new file *)
+Definition compute_unchecked {b A} `{WithDefault A} : (Is_true b -> A) -> A :=
+  if b as b return (Is_true b -> _) -> _
+  then fun f => f I
+  else fun _ => default.
+
+Lemma compute_unchecked_eq {b A}  `{WithDefault A} (f : Is_true b -> A) Hb
+  : compute_unchecked f = f Hb.
+Proof.
+  revert f Hb;
+    destruct b; cbn;
+    try tauto.
+  destruct Hb; tauto.
+Qed.
 
 (* TODO: move these hints to coqutil *)
 
