src/Utils/SpacedMapTreeN.v
@@ -4,27 +4,6 @@ From coqutil Require Import Map.Interface.
 
 From Utils Require Import Booleans Default Base Eqb Options ExtraMaps Monad MapTreeN.
 From Utils Require TrieMap.
-
-(*TODO: move to Booleans or a new file *)
-Definition compute_checked {b A} : (Is_true b -> A) -> option A :=
-  if b as b return (Is_true b -> _) -> _
-  then fun f => Some (f I)
-  else fun _ => None.
-
-(*TODO: move to Booleans or a new file *)
-Definition compute_unchecked {b A} `{WithDefault A} : (Is_true b -> A) -> A :=
-  if b as b return (Is_true b -> _) -> _
-  then fun f => f I
-  else fun _ => default.
-
-Lemma compute_unchecked_eq {b A}  `{WithDefault A} (f : Is_true b -> A) Hb
-  : compute_unchecked f = f Hb.
-Proof.
-  revert f Hb;
-    destruct b; cbn;
-    try tauto.
-  destruct Hb; tauto.
-Qed.
   
 Section __.
   Context {key} {m : forall A, map.map key A}.
